

Reinforcement Learning

Assignment 1 (Theoretical Questions)

Group Members

Matheus da Silva Araujo – ID!!!

Miguel Ángel Carrillo – ID!!!

January 22, 2026

Problem Statement

Application of the Lai–Robbins bound. The asymptotic lower bound on the total regret L_T for any consistent bandit algorithm is given by the Lai–Robbins bound:

$$\liminf_{T \rightarrow \infty} \frac{\mathbb{E}[L_T]}{\ln T} \geq \sum_{a: \Delta_a > 0} \frac{\Delta_a}{D_{\text{KL}}(P_a \parallel P_*)},$$

where D_{KL} is the Kullback–Leibler divergence between the distribution of a suboptimal arm a (P_a) and the optimal arm (P_*), and Δ_a is the gap in expected reward between the optimal arm and arm a .

1 Question 1

Derive the explicit formula for the KL-divergence between two Bernoulli distributions with parameters p and q :

$$D_{\text{KL}}(\text{Ber}(p) \parallel \text{Ber}(q)).$$

Derivation:

General expression for KL-divergence between distributions $r(x)$ and $s(x)$ with discrete random variables:

$$D_{\text{KL}}(r(x) \parallel s(x)) = \sum_{x \in X} r(x) \log \left(\frac{r(x)}{s(x)} \right) \quad (1)$$

Expression for a Bernoulli distribution with parameter p :

$$P(X = x) = \begin{cases} 1 - p, & \text{if } X = 0 \\ p, & \text{if } X = 1 \end{cases}$$

Combining both expressions:

$$\begin{aligned}
D_{\text{KL}}(\text{Ber}(p) \parallel \text{Ber}(q)) &= \sum_{x \in X=\{0,1\}} P(X=x) \log \left(\frac{P(X=x)}{Q(X=x)} \right) \\
&= P(X=0) \log \left(\frac{P(X=0)}{Q(X=0)} \right) + P(X=1) \log \left(\frac{P(X=1)}{Q(X=1)} \right) \\
&= (1-p) \log \left(\frac{1-p}{1-q} \right) + p \log \left(\frac{p}{q} \right).
\end{aligned}$$

Final Answer

$$D_{\text{KL}}(\text{Ber}(p) \parallel \text{Ber}(q)) = (1-p) \log \left(\frac{1-p}{1-q} \right) + p \log \left(\frac{p}{q} \right).$$

2 Question 2

Same question for two Gaussian distributions sharing the same variance.

Derivation:

General expression for Gaussian distribution with variance σ^2 and mean μ :

$$\mathcal{N}(x, \mu, \sigma) = \frac{1}{\sqrt{2\pi}\sigma} \exp\left(-\frac{(x-\mu)^2}{2\sigma^2}\right)$$

Assuming without loss of generality that the two Gaussian distributions have different means, $P(X, \mu_1, \sigma), Q(X, \mu_2, \sigma)$.

General expression for KL-divergence between distributions $R(x)$ and $S(x)$ with continuous random variables:

$$D_{\text{KL}}(R(x) \parallel S(x)) = \int_{-\infty}^{+\infty} R(x) \log \left(\frac{R(x)}{S(x)} \right) dx = \mathbb{E}_{X \sim R} \left[\log \left(\frac{R(X)}{S(X)} \right) \right] \quad (2)$$

where \mathbb{E} is the expected value.

Analyzing the log-term isolated first:

$$\begin{aligned}
\log \frac{P(x)}{Q(x)} &= \log P(x) - \log Q(x) \\
&= \log \left[\left(\frac{1}{\sqrt{2\pi}\sigma^2} \right) \exp \left(\frac{(x-\mu_1)^2}{2\sigma^2} \right) \right] - \log \left[\left(\frac{1}{\sqrt{2\pi}\sigma^2} \right) \exp \left(\frac{(x-\mu_2)^2}{2\sigma^2} \right) \right] \\
&= \log \left(\frac{1}{\sqrt{2\pi}\sigma^2} \right) - \frac{(x-\mu_1)^2}{2\sigma^2} - \log \left(\frac{1}{\sqrt{2\pi}\sigma^2} \right) + \frac{(x-\mu_2)^2}{2\sigma^2} \\
&= \frac{(x-\mu_2)^2 - (x-\mu_1)^2}{2\sigma^2} \\
&\rightarrow \log \frac{P(x)}{Q(x)} = \frac{(x-\mu_2)^2 - (x-\mu_1)^2}{2\sigma^2} \quad (3)
\end{aligned}$$

Analyzing the numerator of Equation 3:

$$\begin{aligned}
(x - \mu_2)^2 - (x - \mu_1)^2 &= (x^2 - 2x\mu_2 + \mu_2^2) - (x^2 - 2x\mu_1 + \mu_1^2) \\
&= 2x(\mu_1 - \mu_2) + \mu_2^2 - \mu_1^2 \\
&= 2x(\mu_1 - \mu_2) + (\mu_2 - \mu_1)(\mu_2 + \mu_1) \\
&= (\mu_1 - \mu_2)(2x - \mu_2 - \mu_1)
\end{aligned}$$

$$\rightarrow (x - \mu_2)^2 - (x - \mu_1)^2 = (\mu_1 - \mu_2)(2x - \mu_2 - \mu_1) \quad (4)$$

Substituting Equations 4 into the numerator of 3:

$$\log \frac{P(x)}{Q(x)} = \frac{(\mu_1 - \mu_2)(2x - \mu_1 - \mu_2)}{2\sigma^2} \quad (5)$$

Then, from the expected value definition of KL-divergence and Equation 5, it follows that

$$\begin{aligned}
D_{\text{KL}}(P(x) \parallel Q(x)) &= \mathbb{E}_{X \sim P} \left[\log \left(\frac{P(X)}{Q(X)} \right) \right] \\
&= \mathbb{E}_{X \sim P} \left[\frac{(\mu_1 - \mu_2)(2X - \mu_1 - \mu_2)}{2\sigma^2} \right] \\
&= \frac{(\mu_1 - \mu_2)}{2\sigma^2} \mathbb{E}_{X \sim P} [2X - \mu_1 - \mu_2].
\end{aligned} \quad (6)$$

Finally, from the linearity of expectation ($\mathbb{E}[aX + b] = a\mathbb{E}[X] + b$) and the information that $P(X)$ is a Gaussian distribution (implying that $\mathbb{E}_{X \sim P} = \mu_1$), applied to Equation 6:

$$\begin{aligned}
D_{\text{KL}}(P(x) \parallel Q(x)) &= \frac{(\mu_1 - \mu_2)}{2\sigma^2} \mathbb{E}_{X \sim P} [(2X - \mu_1 - \mu_2)] \\
&= \frac{(\mu_1 - \mu_2)}{2\sigma^2} (2\mu_1 - \mu_1 - \mu_2) \\
&= \frac{(\mu_1 - \mu_2)}{2\sigma^2} (\mu_1 - \mu_2) \\
&= \frac{(\mu_1 - \mu_2)^2}{2\sigma^2}
\end{aligned}$$

$$\begin{aligned}
\rightarrow D_{\text{KL}}(P(X, \mu_1, \sigma)(X) \parallel Q(X, \mu_2, \sigma)(X)) &= \\
&= \frac{(\mu_1 - \mu_2)^2}{2\sigma^2}
\end{aligned}$$

Answer

$$D_{\text{KL}}(P(X, \mu_1, \sigma)(X) \parallel Q(X, \mu_2, \sigma)(X)) = \frac{(\mu_1 - \mu_2)^2}{2\sigma^2} \quad (7)$$

3 Question 3

Show that for the Bernoulli bandit, it is “easier” (i.e., theoretically implies lower regret) to distinguish an arm with mean $p = 0.9$ from an optimal arm with $p_ = 0.99$ than it is to distinguish an arm with $p = 0.55$ from an optimal arm with $p_* = 0.64$, even though the difference in means is identical ($\Delta = 0.09$) in both cases. What about the Gaussian case?*

Answer

Bernoulli case:

Gaussian case: